prove steal?

theories/code.v
@@ -5,21 +5,22 @@ From iris.program_logic Require Import atomic.
 From iris.proofmode Require Import proofmode.
 From iris.heap_lang Require Import proofmode notation.
 From iris.prelude Require Import options.
-From chase_lev Require Import helpers.
+From chase_lev Require Import helpers mono_list.
+
+Definition CAP_CONST : nat := 10.
 
 (*
   We use a finite length list without resizing;
   The push function diverges if bot gets out of bound.
   +--+--+--+--+--+--+--+--
-  |  |10|20|30|40|  |  |   ..
+  |99|10|20|30|40|  |  |   ..
   +--+--+--+--+--+--+--+--
       ^           ^
       |           |
-      top (steal) bot (push, pop)
+      top         bot
 *)
 
 Section code.
-  Definition CAP_CONST : nat := 10.
   Definition new_deque : val :=
     λ: <>,
       let: "array" := AllocN #CAP_CONST #0 in
@@ -58,90 +59,99 @@ Section code.
   (* NOTE: b ≤ t doesn't necessarily mean the deque was empty!
     It can also be the case that there was one element and
     the owner thread prematurely decremented b trying to pop. *)
+  (* TODO: change to NONE/SOME *)
   Definition steal : val :=
     λ: "deque",
       let: "array" := arr "deque" in
       let: "t" := !(top "deque") in
       let: "b" := !(bot "deque") in
-      if: "b" ≤ "t" then #()
-      else if: CAS (top "deque") "t" ("t" + #1) then !("array" +ₗ "t")
-      else #().
+      if: "b" ≤ "t" then (#false, #())
+      else if: CAS (top "deque") "t" ("t" + #1)
+      then (#true, !("array" +ₗ "t"))
+      else (#false, #()).
 End code.
 
 Class dequeG Σ := DequeG {
     deque_tokG :> ghost_varG Σ (list val);
+    mono_listG :> mono_listG val Σ;
     mono_natG :> mono_natG Σ
   }.
 Definition dequeΣ : gFunctors :=
   #[ghost_varΣ (list val);
+    mono_listΣ val;
     mono_natΣ
   ].
 Global Instance subG_dequeΣ {Σ} : subG dequeΣ Σ → dequeG Σ.
 Proof. solve_inG. Qed.
 
-(* TODO: move this to helpers.v *)
-Section Inbound.
-  Definition deque_bound (t b : nat) (l : list val) :=
-    t ≤ b /\ b < length l /\ length l = CAP_CONST.
-
-  Lemma deque_bound_init : deque_bound 0 0 (replicate (Z.to_nat CAP_CONST) #0).
-  Proof.
-    unfold deque_bound. repeat split; auto.
-    rewrite replicate_length. replace (Z.to_nat CAP_CONST) with 10 by auto. lia.
-  Qed.
-
-  Lemma deque_bound_2_length t1 b1 t2 b2 l1 l2 :
-    deque_bound t1 b1 l1 → deque_bound t2 b2 l2 → length l1 = length l2.
-  Admitted.
-
-  Lemma deque_bound_insert t b l i v :
-    deque_bound t b l → i < length l → deque_bound t b (<[b:=v]> l).
-  Admitted.
-
-  Lemma deque_bound_extend_right t b l :
-    deque_bound t b l → b < length l → deque_bound t (S b) l.
-  Admitted.
-
-  Lemma deque_bound_shrink_left t b l : 
-    deque_bound t b l → t < b → deque_bound (S t) b l.
-  Admitted.
-End Inbound.
-
 Section RA.
   Context `{!heapGS Σ, !dequeG Σ} (N : namespace).
   Notation iProp := (iProp Σ).
 
-  (* TODO [URGENT]: we actually need mono_list of [0..t), not just mono_nat of t *)
-  Definition mono_toparr (γt : gname) (t : nat) (l : list val) : iProp :=
-    let tl := match l with | [] => (2*t) | _ => (2*t+1) end in
-    mono_nat_auth_own γt 1 tl.
+  Definition mono_deque_auth_own (γm : gname) (l : list val) (t b : nat) : iProp :=
+    ∃ (γl γmb : gname),
+    ⌜γm = encode (γl, γmb)⌝ ∗
+    ⌜deque_bound t b l⌝ ∗
+    mono_list_auth_own γl 1 (take t l) ∗
+    mono_nat_auth_own γmb 1 (
+      2 * t + (if decide(t < b) then 1 else 0)
+    ).
 
-  Definition mono_toparr_lb (γt : gname) (t : nat) (l : list val) : iProp :=
-    let tl := match l with | [] => (2*t) | _ => (2*t+1) end in
-    mono_nat_lb_own γt tl.
+  Definition mono_deque_lb_own (γm : gname) (l : list val) (t b : nat) : iProp :=
+    ∃ (γl γmb : gname),
+    ⌜γm = encode (γl, γmb)⌝ ∗
+    ⌜deque_bound t b l⌝ ∗
+    mono_list_lb_own γl (take t l) ∗
+    mono_nat_lb_own γmb (
+      2 * t + (if decide(t < b) then 1 else 0)
+    ).
 
-  Lemma mono_toparr_get_lb (γt : gname) (t : nat) (l : list val) :
-    mono_toparr γt t l ==∗ mono_toparr γt t l ∗ mono_toparr_lb γt t l.
+  Lemma mono_deque_own_alloc l :
+    ⌜length l = CAP_CONST⌝ ==∗ ∃ γ, mono_deque_auth_own γ l 0 0.
+  Proof.
+    iIntros (H).
+    iMod (mono_list_own_alloc []) as (γl) "[L _]".
+    iMod (mono_nat_own_alloc 0) as (γmb) "[N _]".
+    iExists (encode (γl, γmb)). iModIntro.
+    iExists _,_. iSplit; iFrame; auto.
+    iPureIntro. by apply deque_bound_init.
+  Qed.
+
+  Lemma mono_deque_get_lb γm l t b :
+    mono_deque_auth_own γm l t b ==∗ mono_deque_auth_own γm l t b ∗ mono_deque_lb_own γm l t b.
   Proof.
   Admitted.
 
-  Lemma mono_toparr_lb_own_top (γt : gname) (t1 t2 : nat) (l1 l2 : list val) :
-    mono_toparr γt t1 l1 -∗ mono_toparr_lb γt t2 l2 -∗ ⌜t2 ≤ t1⌝.
+  Lemma mono_deque_auth_lb γm l1 t1 b1 l2 t2 b2 :
+    mono_deque_auth_own γm l1 t1 b1 -∗ mono_deque_lb_own γm l2 t2 b2 -∗
+    ⌜t2 ≤ t1 ∧ take t2 l2 = take t2 l1⌝.
   Proof.
   Admitted.
-
-  Lemma mono_toparr_append (γt : gname) (l1 l2 : list val) (t : nat) :
-    mono_toparr γt t l1 ==∗ mono_toparr γt t (l1 ++ l2).
+(*
+  Lemma mono_deque_append (γm : gname) (l1 l2 : list val) (t : nat) :
+    mono_deque_auth_own γm t l1 ==∗ mono_deque_auth_own γm t (l1 ++ l2).
   Proof.
     iIntros "mta". destruct l2. { rewrite app_nil_r. auto. }
-    destruct l1; last first. { unfold mono_toparr. auto. }
-    unfold mono_toparr. simpl.
+    destruct l1; last first. { unfold mono_deque. auto. }
+    unfold mono_deque. simpl.
     iMod (mono_nat_own_update (t+(t+0)+1) with "mta") as "[mta _]"; auto. lia.
   Qed.
 
-  Lemma mono_toparr_top (γt : gname) (t1 t2 : nat) (l1 l2 : list val) :
+  Lemma mono_deque_top (γm : gname) (t1 t2 : nat) (l1 l2 : list val) :
     t1 ≤ t2 →
-    mono_toparr γt t1 l1 ==∗ mono_toparr γt t2 l2.
+    mono_deque_auth_own γm t1 l1 ==∗ mono_deque_auth_own γm t2 l2.
+  Admitted.
+  *)
+
+  Lemma mono_deque_top_nonempty γm t l1 b1 l2 b2 :
+    t < b2 →
+    mono_deque_auth_own γm l1 t b1 -∗ mono_deque_lb_own γm l2 t b2 -∗
+    ⌜t < b1⌝.
+  Admitted.
+
+  Lemma mono_deque_update_top γm t2 l t1 b :
+    t1 ≤ t2 →
+    mono_deque_auth_own γm l t1 b ==∗ mono_deque_auth_own γm l t2 b.
   Admitted.
 End RA.
 
@@ -153,19 +163,19 @@ Section proof.
 
   (* TODO: change l to ↦∗{#1} & make another ghost_var in deque_content?
      (see msqueue) *)
-  Definition deque_inv (γq γt : gname) (arr top bot : loc) : iProp :=
+  Definition deque_inv (γq γm : gname) (arr top bot : loc) : iProp :=
     ∃ (t b : nat) (l : list val),
+      ⌜deque_bound t b l⌝ ∗
       top ↦ #t ∗ bot ↦{#1/2} #b ∗ arr ↦∗{#1/2} l ∗
       ghost_var γq (1/2) (slice l t b) ∗
-      mono_toparr γt t (slice l t b) ∗
-      ⌜deque_bound t b l⌝.
+      mono_deque_auth_own γm l t b.
 
-  Definition is_deque (γq γt : gname) (q : val) : iProp :=
+  Definition is_deque (γq γm : gname) (q : val) : iProp :=
     ∃ (arr top bot : loc),
       ⌜q = (#arr, #top, #bot)%V⌝ ∗
-      inv dequeN (deque_inv γq γt arr top bot).
-  Global Instance is_deque_persistent γq γt q :
-    Persistent (is_deque γq γt q) := _.
+      inv dequeN (deque_inv γq γm arr top bot).
+  Global Instance is_deque_persistent γq γm q :
+    Persistent (is_deque γq γm q) := _.
 
   Definition deque_content (γq : gname) (frag : list val) : iProp :=
     ghost_var γq (1/2) frag.
@@ -186,11 +196,12 @@ Section proof.
   Ltac autoall :=
     auto; try by (unfold deque_bound in *; unfold CAP_CONST in *; lia).
 
+    (*
   Lemma new_deque_spec :
     {{{ True }}}
       new_deque #()
-    {{{ γq γt q, RET q;
-      is_deque γq γt q ∗ deque_content γq [] ∗
+    {{{ γq γm q, RET q;
+      is_deque γq γm q ∗ deque_content γq [] ∗
       own_deque γq q
     }}}.
   Proof with autoall.
@@ -198,9 +209,9 @@ Section proof.
     wp_lam. wp_alloc arr as "[arr↦1 arr↦2]"...
     wp_pures. wp_alloc b as "[b↦1 b↦2]". wp_alloc t as "t↦".
     iMod (ghost_var_alloc []) as (γq) "[γ1 γ2]".
-    iMod (mono_nat_own_alloc 0) as (γt) "[γt _]".
-    iMod (inv_alloc dequeN _ (deque_inv γq γt arr t b)
-      with "[t↦ b↦1 arr↦1 γ1 γt]") as "Inv".
+    iMod (mono_deque_own_alloc) as (γm) "γm".
+    iMod (inv_alloc dequeN _ (deque_inv γq γm arr t b)
+      with "[t↦ b↦1 arr↦1 γ1 γm]") as "Inv".
     { iNext. iExists 0, 0, _. iFrame "t↦ b↦1 arr↦1". iFrame.
       iPureIntro. apply deque_bound_init. }
     wp_pures. iModIntro. iApply "HΦ". iSplit.
@@ -208,8 +219,8 @@ Section proof.
     - iSplitR "b↦2 arr↦2"... iExists _,_,_,0,_. iFrame...
   Qed.
 
-  Lemma push_spec γq γt q (v : val) :
-    is_deque γq γt q -∗
+  Lemma push_spec γq γm q (v : val) :
+    is_deque γq γm q -∗
     own_deque γq q -∗
     <<< ∀∀ l : list val, deque_content γq l >>>
       push q v @ ↑N
@@ -267,7 +278,7 @@ Section proof.
     iDestruct "b↦" as "[b↦ b👑]".
     iMod (ghost_var_update_2 (slice (<[b:=v]> l) t3 (S b))
       with "γ Cont") as "[γ Cont]". { rewrite Qp.half_half... }
-    iMod (mono_toparr_append _ (slice (<[b:=v]> l) t3 b) [v] with "mta") as "mta".
+    iMod (mono_deque_append _ (slice (<[b:=v]> l) t3 b) [v] with "mta") as "mta".
       rewrite <- slice_extend_right... 2: rewrite list_lookup_insert...
     iMod ("Commit" with "[Cont b👑 arr👑]") as "Φ".
     { iFrame. iExists _,_,_,(S b),_; iFrame. iSplit... rewrite insert_length... }
@@ -277,17 +288,16 @@ Section proof.
     iFrame "t↦ b↦ arr↦ γ". iSplit...
     iPureIntro. apply deque_bound_extend_right...
   Qed.
+  *)
 
-  Lemma steal_spec γq γt q :
-    is_deque γq γt q -∗
+  Lemma steal_spec γq γm q :
+    is_deque γq γm q -∗
     <<< ∀∀ l : list val, deque_content γq l >>>
-      steal q @ ↑N
-    <<< ∃∃ (l' : list val) (v : val),
-      deque_content γq l' ∗
-      match v with
-      | #() => ⌜l' = l⌝
-      | _ => ⌜l = [v] ++ l'⌝
-      end, RET v >>>.
+      steal q @ ↑dequeN
+    <<< ∃∃ (l' : list val) (b : bool) (v : val),
+        deque_content γq l' ∗
+        ⌜l = if b then [v]++l' else l'⌝ ,
+      RET (#b, v) >>>.
   Proof with autoall.
     iIntros "#Is" (Φ) "AU".
       iDestruct "Is" as (arr top bot) "[%Is Inv]". subst.
@@ -295,49 +305,73 @@ Section proof.
 
     (* load top *)
     wp_bind (! _)%E.
-    iInv "Inv" as (t1 b1 l1) ">(t↦ & b↦ & arr↦ & γ & mta & %BOUND1)".
-      iMod (mono_toparr_get_lb with "mta") as "[mta #mtlb1]".
+    iInv "Inv" as (t1 b1 l1) ">(%BOUND1 & t↦ & b↦ & arr↦ & γ & MD)".
+      iMod (mono_deque_get_lb with "MD") as "[MD #MDlb1]".
     wp_load.
-    iModIntro. iSplitL "t↦ b↦ arr↦ γ mta".
+    iModIntro. iSplitL "t↦ b↦ arr↦ γ MD".
       { iExists _,_,_. iFrame "t↦ b↦ arr↦ γ"... }
     wp_pures.
 
     (* load bot *)
     wp_bind (! _)%E.
-    iInv "Inv" as (t2 b2 l2) ">(t↦ & b↦ & arr↦ & γ & mta & %BOUND2)".
-      iMod (mono_toparr_get_lb with "mta") as "[mta #mtlb2]".
-      iDestruct (mono_toparr_lb_own_top with "mta mtlb1") as "%Ht12".
+    iInv "Inv" as (t2 b2 l2) ">(%BOUND2 & t↦ & b↦ & arr↦ & γ & MD)".
+      iMod (mono_deque_get_lb with "MD") as "[MD #MDlb2]".
+      iDestruct (mono_deque_auth_lb with "MD MDlb1") as "[%Ht12 %HL12]".
     wp_load.
-    iModIntro. iSplitL "t↦ b↦ arr↦ γ mta".
+    iModIntro. iSplitL "t↦ b↦ arr↦ γ MD".
       { iExists _,_,_. iFrame "t↦ b↦ arr↦ γ"... }
     wp_pures.
 
     (* no chance to steal *)
     case_bool_decide; wp_pures.
-    { admit. }
+    { iMod "AU" as (l) "[Cont [_ Commit]]".
+      iMod ("Commit" $! l false #() with "[Cont]")... }
 
     (* cas top *)
     wp_bind (CmpXchg _ _ _)%E.
-    iInv "Inv" as (t3 b3 l3) ">(t↦ & b↦ & arr↦ & γ & mta & %BOUND3)".
-      iDestruct (mono_toparr_lb_own_top with "mta mtlb2") as "%Ht23".
+    iInv "Inv" as (t3 b3 l3) ">(%BOUND3 & t↦ & b↦ & arr↦ & γ & MD)".
+      iDestruct (mono_deque_auth_lb with "MD MDlb2") as "[%Ht23 %HL23]".
     destruct (decide (t3 = t1)).
     - (* success *)
       assert (t1 = t2)... subst. wp_cmpxchg_suc.
-      assert (t2 < b3) by admit.
+        clear Ht12 Ht23.
+      (* update ghost *)
+      iDestruct (mono_deque_top_nonempty _ with "MD MDlb2") as "%Htb23"...
       replace (Z.of_nat t2 + 1)%Z with (Z.of_nat (S t2))...
-      iMod (mono_toparr_top _ _ t2 (S t2) with "mta") as "mta"...
+      iMod (mono_deque_update_top _ _ (S t2) with "MD") as "MD"...
+      iMod (mono_deque_get_lb with "MD") as "[MD #MDlb3]".
+      (* AU *)
       iMod "AU" as (l') "[Cont [_ Commit]]".
         unfold deque_content.
         iDestruct (ghost_var_agree with "γ Cont") as "%". subst.
-        iMod (ghost_var_update_2 (slice l3 (S t2) b3) with "γ Cont") as "[γ Cont]".
-          { rewrite Qp.half_half... }
+        iMod (ghost_var_update_2 (slice l3 (S t2) b3) with "γ Cont")
+          as "[γ Cont]". { rewrite Qp.half_half... }
         assert (is_Some (l3 !! t2)) as [k HLk].
           { rewrite lookup_lt_is_Some... }
-        iMod ("Commit" $! _ k with "[Cont]").
-          { iFrame. admit. }
-      iModIntro. iSplitL "t↦ b↦ arr↦ γ mta".
-        { iExists _,_,_. iFrame "t↦ b↦ arr↦ γ mta".
+        iMod ("Commit" $! (slice l3 (S t2) b3) true k with "[Cont]").
+          { iFrame. erewrite slice_shrink_left... }
+      iModIntro. iSplitL "t↦ b↦ arr↦ γ MD".
+        { iExists _,_,_. iFrame "t↦ b↦ arr↦ γ MD".
           iNext. iPureIntro. apply deque_bound_shrink_left... }
       wp_pures.
+      (* load arr[t2] *)
+      wp_bind (! _)%E.
+      iInv "Inv" as (t4 b4 l4) ">(%BOUND4 & t↦ & b↦ & arr↦ & γ & MD)".
+        iDestruct (mono_deque_auth_lb with "MD MDlb3") as "[%Ht34 %HL34]".
+      assert (l4 !! t2 = Some k).
+        { rewrite -(lookup_take _ (S t2))... rewrite -HL34 lookup_take... }
+      iApply (wp_load_offset with "arr↦")... 1: eauto.
+      iNext. iIntros "arr↦".
+      iModIntro. iSplitL "t↦ b↦ arr↦ γ MD".
+      { iExists _,_,_. iFrame "t↦ b↦ arr↦ γ MD"... }
+      by wp_pures.
+    - (* fail *)
+      wp_cmpxchg_fail. { intro. injection H0... }
+      iMod "AU" as (l) "[Cont [_ Commit]]".
+      iMod ("Commit" $! l false #() with "[Cont]")...
+      iModIntro. iSplitL "t↦ b↦ arr↦ γ MD".
+      { iExists _,_,_. iFrame "t↦ b↦ arr↦ γ MD"... }
+      by wp_pures.
+  Unshelve. (* what namespace?? *)
   Admitted.
 End proof.
